updates_from_cpp (#40)
integrating with AssemblyCache and Processor

Reviewed-on: https://www0.sbclab.net/gitea/eLyKseeR/elykseer-ml/pulls/40

bin/lxr_backup.ml
@@ -2,11 +2,8 @@
 
 open Elykseer__Lxr
 open Elykseer__Lxr.Configuration
-open Elykseer__Lxr.Environment
 
 open Elykseer_utils
-
-open Mlcpp_cstdio
 
 let def_myid = "1234567890"
 
@@ -16,7 +13,6 @@ let arg_files = ref []
 let arg_dbpath = ref "/tmp/db"
 let arg_chunkpath = ref "lxr"
 let arg_nchunks = ref 16
-let arg_nproc = ref 1
 let arg_myid = ref def_myid
 
 let argspec =
@@ -26,150 +22,54 @@ let argspec =
     ("-x", Arg.Set_string arg_chunkpath, "sets output path for encrypted chunks");
     ("-d", Arg.Set_string arg_dbpath, "sets database path");
     ("-n", Arg.Set_int arg_nchunks, "sets number of chunks (16-256) per assembly");
-    ("-j", Arg.Set_int arg_nproc, "sets number of parallel processes");
     ("-i", Arg.Set_string arg_myid, "sets own identifier");
   ]
 
 let anon_args_fun fn = arg_files := fn :: !arg_files
 
-(** the minimum available size in an assembly *)
-(* let aminsz = 127 *)
-
-let curr_assembly_sz n = Conversion.n2i (Assembly.assemblysize n)
-
-(* data structure of a backup plan *)
-type backup_plan_file = {
-  fhash : string;
-  curfi : Filesupport.fileinformation;
-  curbs : BackupPlanner.fileblock list;
-  reffi : Filesupport.fileinformation option;
-  refbs : (Assembly.blockinformation list) option
-}
-type backup_plan = {
-  bp : backup_plan_file list
-}
-
-let plan_backup e0 fns =
-  let a = e0.cur_assembly in
-  let afree = curr_assembly_sz a.nchunks - (Conversion.n2i a.apos) in
-  let%lwt relfiles = Relfiles.new_map e0.config in
-  let%lwt (_anum', _afree', bpfs) = Lwt_list.fold_left_s (fun (anum,afree,acc) fn ->
-        let fhash = Elykseer_crypto.Sha256.string fn in
-        let ((anum',afree'),fbs) = BackupPlanner.analyse_file a.nchunks afree anum fn in
-        let%lwt ref = Relfiles.find fhash relfiles in
-        let oreffi = match ref with None -> None | Some r -> Some r.rfi in
-        let orefbs = match ref with None -> None | Some r -> Some r.rfbs in
-        Lwt.return (anum', afree', {fhash = fhash; curfi = fbs.fbifi; curbs = fbs.fbifblocks; reffi = oreffi; refbs = orefbs } :: acc)
-      ) (Conversion.i2p 1, Conversion.i2n afree, []) fns in
-    Lwt.return {bp = List.rev bpfs}
-
-let execute_backup_fileblock e _anum (fname,blocks) =
-  Cstdio.File.fopen fname "rx" |> function
-    | Ok fptr ->
-      let backup_block e0 fptr fb =
-          let fpos = BackupPlanner.fbfpos fb in
-          Cstdio.File.fseek fptr (Conversion.n2i fpos) |> function
-            | Ok _ -> begin
-              let sz = Conversion.n2i fb.fbsz in
-              let buf = Cstdio.File.Buffer.create sz in
-              Cstdio.File.fread buf sz fptr |> function
-                | Ok _nread ->
-                  let bplain = Elykseer__Lxr.Cstdio.BufferPlain.from_buffer buf in
-                  let (_apos, newe) = EnvironmentWritable.backup e0 fname fpos bplain in newe
-                | Error (errno,errstr) -> 
-                  Printf.printf "read error no:%d err:%s\n" errno errstr; e0
-              end
-            | Error (errno,errstr) -> 
-                Printf.printf "seek error no:%d err:%s\n" errno errstr; e0
-      in
-      let e1 = List.fold_left (fun env fb -> backup_block env fptr fb) e blocks in
-      Cstdio.File.fclose fptr |> ignore;
-      e1
-    | Error (errno,errstr) -> 
-        Printf.printf "open error no:%d err:%s\n" errno errstr |> ignore; e
-
-let extract_fileblocks anum (bp : backup_plan) =
-  List.map (fun bpf -> let fname = bpf.curfi.fname in
-    (fname, List.filter (fun fbs -> BackupPlanner.fbanum fbs = anum) bpf.curbs)
-  ) bp.bp
-
-let rec run_backup_for_assembly e0 pid anum acount (bp : backup_plan) =
-  if anum > acount then e0
-  else begin
-      (* Printf.printf "executing backup of assembly %d\n" anum; *)
-      let anum_p = Conversion.i2p anum in
-      let fileblocks' = extract_fileblocks anum_p bp in
-      let e1 = List.fold_left (fun env fb -> execute_backup_fileblock env anum fb) e0 fileblocks' in
-      let e2 = Environment.EnvironmentWritable.finalise_and_recreate_assembly e1 in
-      run_backup_for_assembly e2 pid (anum + 1) acount bp
-  end
-
-(* let start_processes n =
-  let rec start_processes' acc n =
-    if n = 0
-      then List.rev acc
-      else
-        let proc = n in  (* TODO create external process *)
-        start_processes' (proc :: acc) (n - 1) in
-  start_processes' [] n *)
-
-let run_distributed_backup e0 nproc acount bp =
-  (* start n processes *)
-  let ps = (* start_processes *) nproc in
-  (* distribute work among processes *)
-  run_backup_for_assembly e0 ps 1 acount bp
-
-let validate_fileblocks fname fhash bis =
-    if !arg_verbose then
-      let list_sum = List.fold_left (+) 0 in
-      let nb = List.length bis in
-      let na = List.map (fun (e : Assembly.blockinformation) -> e.blockaid) bis |> List.sort_uniq compare |> List.length in
-      let sumbsz = List.map (fun (e : Assembly.blockinformation) -> Conversion.n2i e.blocksize) bis |> list_sum in
-      let lbsz = List.map (fun (e : Assembly.blockinformation) -> (Conversion.n2i e.filepos, Conversion.n2i e.blocksize)) bis |>
-                 List.sort (fun e1 e2 -> compare (fst e1) (fst e2)) in
-      (* let%lwt () = Lwt_list.iteri_s (fun i (a,b) -> Lwt_io.printlf "    %d: %d + %d" i a b) lbsz in *)
-      let sumdelta = Zip.zip (lbsz) (List.tl lbsz) |> List.map (fun ((a,b),(a',_b')) -> (a' - a) - b) |> list_sum in
-      let (res,res') = if 0 = sumdelta then ("+","✅") else ("-","❌") in
-      Lwt_io.printlf "%s%s '%s' (%s) in %d assemblies with %d blocks, %d bytes in total (control=%d)" res res' fname fhash na nb sumbsz sumdelta
-    else Lwt.return ()
-
-let output_rel_files e (bp : backup_plan) =
-  let fbis = Env.consolidate_files e.fblocks.entries in
+let output_rel_files config (fiset : Filesupport.fileinformation list) (fbstore : Store.FBlockListStore.coq_R) =
+  let fbis = Env.consolidate_files fbstore.entries in
   if !arg_dryrun then
-    Lwt_list.iter_s (fun (fname, bis) -> let fhash = Elykseer_crypto.Sha256.string fname in
-                       let%lwt () = validate_fileblocks fname fhash bis in
-                       let%lwt () = Lwt_io.printlf "%s" fhash in
+    Lwt_list.iter_s (fun (fhash, bis) ->
+                       let%lwt () = Lwt_io.printlf "fhash = %s" fhash in
+                       let%lwt _ = Lwt_list.iter_s (fun (fi : Filesupport.fileinformation) ->
+                        Lwt_io.printlf " %s %d %s %d %s %s" fi.fname
+                                                       (Conversion.n2i fi.fsize)
+                                                       fi.fowner
+                                                       (Conversion.n2i fi.fpermissions)
+                                                       fi.fmodified
+                                                       fi.fchecksum
+                        )
+                        (fiset) in
                        Lwt_list.iter_s (fun (fb : Assembly.blockinformation) ->
-                                          Lwt_io.printlf "  %d@%d=%d %s" (Conversion.p2i fb.blockid)
-                                                                         (Conversion.n2i fb.filepos)
-                                                                         (Conversion.n2i fb.blocksize)
-                                                                         fb.bchecksum
-                                       )
-                                       (List.rev bis)
+                        Lwt_io.printlf "  %d:%d@%d %s" (Conversion.p2i fb.blockid)
+                                                        (Conversion.n2i fb.blocksize)
+                                                        (Conversion.n2i fb.filepos)
+                                                        fb.bchecksum
+                        )
+                        (List.rev bis)
                     ) fbis
   else
-    let%lwt rel = Relfiles.new_map e.config in
-    let%lwt () = Lwt_list.iter_s (fun (fname, bis) -> let fhash = Elykseer_crypto.Sha256.string fname in
-                                    let%lwt () = validate_fileblocks fname fhash bis in
-                                    let bpf = List.find (fun bpf -> bpf.fhash = fhash) bp.bp in
-                                    let%lwt _rel' = Relfiles.add fhash {rfi=bpf.curfi; rfbs=bis} rel in Lwt.return ()) fbis in
+    let%lwt rel = Relfiles.new_map config in
+    let%lwt () = Lwt_list.iter_s (fun (fhash, bis) ->
+                                    let fi = List.find (fun fi -> Elykseer_crypto.Sha256.string (Filesupport.fname fi) = fhash) fiset in
+                                    let%lwt _rel' = Relfiles.add fhash {rfi=fi; rfbs=bis} rel in Lwt.return ()) fbis in
     Relfiles.close_map rel
 
-let output_rel_keys e =
-  let%lwt rel = Relkeys.new_map e.config in
+let output_rel_keys config (kstore : Store.KeyListStore.coq_R) =
+  let%lwt rel = Relkeys.new_map config in
   let%lwt () = Lwt_list.iter_s (fun (aid, ki) ->
-                                let%lwt _ = Relkeys.add aid ki rel in Lwt.return ()) e.keys.entries in
+                                let%lwt _ = Relkeys.add aid ki rel in Lwt.return ()) kstore.entries in
   Relkeys.close_map rel
 
-let output_relations e (bp : backup_plan) =
-  let%lwt () = if !arg_dryrun then Lwt.return () else output_rel_keys e in
-  output_rel_files e bp
+let output_relations fiset (ac : AssemblyCache.assemblycache) =
+  let%lwt () = if !arg_dryrun then Lwt.return () else output_rel_keys ac.acconfig ac.ackstore in
+  output_rel_files ac.acconfig fiset ac.acfbstore
 
 
 let main () = Arg.parse argspec anon_args_fun "lxr_backup: vyxdnji";
   let nchunks = Nchunks.from_int !arg_nchunks in
   if List.length !arg_files > 0
-  && !arg_nproc > 0 && !arg_nproc < 65
   then
     let myid = !arg_myid in
     let conf : configuration = {
@@ -177,22 +77,13 @@ let main () = Arg.parse argspec anon_args_fun "lxr_backup: vyxdnji";
                   path_chunks = !arg_chunkpath;
                   path_db     = !arg_dbpath;
                   my_id       = myid } in
-    let e0 = Environment.EnvironmentWritable.initial_environment conf in
-    let%lwt backup_plan = plan_backup e0 !arg_files in
-    let fcount = List.map (fun bpf -> bpf.fhash) backup_plan.bp |> List.sort_uniq (compare) |> List.length
-    and acount = List.map (fun bpf -> bpf.curbs) backup_plan.bp |> List.map (List.map BackupPlanner.fbanum) |>
-                              List.flatten |> List.sort_uniq (compare) |> List.length in
-    let%lwt () = Lwt_io.printlf "backup of %d %s in %d %s" fcount (Utils.pluralise "file" fcount) acount (Utils.pluralise2 "assembly" "assemblies" acount) in
-    let%lwt () = let rcount = List.map (fun bpf -> match bpf.refbs with None -> [] | Some ls -> ls) backup_plan.bp |>
-                              List.map (List.map Assembly.blockaid) |>
-                              List.flatten |> List.sort_uniq (compare) |> List.length in
-                 Lwt_io.printlf "reference contains %d %s" rcount (Utils.pluralise2 "assembly" "assemblies" rcount) in
-    let e1 = run_distributed_backup e0 !arg_nproc acount backup_plan in
-    let e2 = Environment.EnvironmentWritable.finalise_assembly e1 in
-    let%lwt () = output_relations e2 backup_plan in
+    let proc = Processor.prepare_processor conf in
+    let (fiset, proc') = List.fold_left (fun (fiset, proc) fp -> let (fi, proc') = Processor.file_backup proc (Filesystem.Path.from_string fp) in (fi :: fiset, proc') ) ([], proc) !arg_files in
+    let proc'' = Processor.close proc' in
+    let%lwt () = output_relations fiset proc''.cache in
     let%lwt () = Lwt_io.printl "done." in
     Lwt.return ()
   else
-    Lwt.return ()
+    Lwt_io.printl "nothing to do."
 
 let () = Lwt_main.run (main ())
