bin/lxr_restore.ml
@@ -2,10 +2,8 @@
 open Elykseer__Lxr
 open Elykseer__Lxr.Configuration
 
-open Elykseer_base.Fsutils
 open Elykseer_utils
 
-open Mlcpp_cstdio
 open Mlcpp_filesystem
 
 let def_myid = "1234567890"
@@ -16,7 +14,6 @@ let arg_dbpath = ref "/tmp/db"
 let arg_chunkpath = ref "lxr"
 let arg_outpath = ref "/tmp/"
 let arg_nchunks = ref 16
-let arg_nproc = ref 1
 let arg_myid = ref def_myid
 
 let argspec =
@@ -26,89 +23,59 @@ let argspec =
     ("-o", Arg.Set_string arg_outpath, "sets output path for restored files");
     ("-d", Arg.Set_string arg_dbpath, "sets database path");
     ("-n", Arg.Set_int arg_nchunks, "sets number of chunks (16-256) per assembly");
-    ("-j", Arg.Set_int arg_nproc, "sets number of parallel processes");
     ("-i", Arg.Set_string arg_myid, "sets own identifier");
   ]
 
 let anon_args_fun fn = arg_files := fn :: !arg_files
 
-let mk_path fp =
-  !arg_outpath ^ "/" ^ fp
-
-let ensure_assembly e relk aid =
-  if (Environment.cur_assembly e |> Assembly.aid) = aid
-    then Lwt.return @@ Ok (Environment.cur_assembly e, Environment.cur_buffer e)
-  else
-  match%lwt Relkeys.find aid relk with
-  | None -> Lwt.return @@ Error "no key found"
-  | Some ki ->
-    let e1 = Environment.EnvironmentReadable.env_add_aid_key aid e ki in
-    match Environment.EnvironmentReadable.restore_assembly e1 aid with
-    | None -> Lwt.return @@ Error "failed to restore assembly"
-    | Some e2 -> Lwt.return @@ Ok (e2.cur_assembly, e2.cur_buffer)
-
-let restore_file_blocks e0 relk fptr (fb : Assembly.blockinformation) =
-  match%lwt ensure_assembly e0 relk fb.blockaid with
-  | Error errstr -> let%lwt () = Lwt_io.printlf "  failed to recall assembly %s with '%s'" fb.blockaid errstr in
-                    Lwt.return (0,e0)
-  | Ok (a,b) ->
-      let sz = Conversion.n2i fb.blocksize in
-      let fbuf = Cstdio.File.Buffer.create sz in
-      let abuf = Elykseer__Lxr.Cstdio.BufferPlain.to_buffer @@ Assembly.id_buffer_t_from_full b in
-      let nread = Elykseer_base.Assembly.get_content ~src:abuf ~sz:sz ~pos:(Conversion.n2i fb.blockapos) ~tgt:fbuf in
-      Cstdio.File.fseek fptr (Conversion.n2i fb.filepos) |> function
-        | Error _ -> let%lwt () = Lwt_io.printlf "  failed to 'fseek'\n" in Lwt.return (0,e0)
-        | Ok _ -> Cstdio.File.fwrite fbuf sz fptr |> function
-          | Error _ -> let%lwt () = Lwt_io.printlf "  failed to 'fwrite'\n" in Lwt.return (0,e0)
-          | Ok _nwritten -> Lwt.return (nread,{ e0 with cur_assembly=a; cur_buffer=b })
-
-let restore_file e0 relf relk fname =
+let restore_file proc relf _relk basep fname =
   let%lwt ofbs = Relfiles.find (Elykseer_crypto.Sha256.string fname) relf in
   match ofbs with
-  | None -> let%lwt () = Lwt_io.printlf "  cannot restore file '%s'" fname in Lwt.return (0,e0)
+  | None -> let%lwt () = Lwt_io.printlf "  cannot restore file '%s'" fname in Lwt.return (0,proc)
   | Some rfbs ->
       let%lwt () = if !arg_verbose then
         Lwt_io.printlf "  restoring %d bytes in file '%s' from %d blocks" (Conversion.n2i rfbs.rfi.fsize) fname (List.length rfbs.rfbs)
         else Lwt.return () in
-      let fout_path = mk_path fname in
-      let dir_path = Filesystem.Path.from_string fout_path |> Filesystem.Path.parent in
-      let%lwt () = if not (Filesystem.Path.exists dir_path) then
-          Filesystem.create_directories dir_path |> function
-          | false -> let%lwt () = Lwt_io.printlf "failed to create directories: %s" fout_path in
-            Lwt.return ()
-          | true -> Lwt.return ()
-        else Lwt.return () in
-      Cstdio.File.fopen fout_path "wx" |> function
-        | Error (errno,errstr) -> let%lwt () = Lwt_io.printf "  fopen returned: %d/%s\n    (filepath '%s')" errno errstr fout_path in Lwt.return (0,e0)
-        | Ok fptr ->
-            let%lwt (cnt,e1) = Lwt_list.fold_left_s (fun (cnt,env) fb -> let%lwt (c',e') = restore_file_blocks env relk fptr fb in Lwt.return(cnt + c',e')) (0,e0) rfbs.rfbs in
-            let () = Cstdio.File.fclose fptr |> ignore in
-            let (res,res') = if rfbs.rfi.fchecksum = fchksum fout_path then ("+","✅") else ("-","❌") in
-            let%lwt () = Lwt_io.printf "%s%s '%s'" res res' fname in
-            let%lwt () = if !arg_verbose then
-                Lwt_io.printlf "    restored with %d bytes in total" cnt
-              else
-                Lwt_io.printl ""
-              in
-            Lwt.return (cnt,e1)
+      let (n, proc') = Processor.file_restore proc basep (Filesystem.Path.from_string fname) rfbs.rfbs in
+      let%lwt _ = Lwt_io.printlf "     -> %d bytes" (Conversion.n2i n) in
+      Lwt.return (Conversion.n2i n, proc')
 
-let ensure_all_available (e : Environment.EnvironmentReadable.coq_E) fns =
-  let%lwt rel = Relfiles.new_map e.config in
-  let%lwt ls = Lwt_list.map_s (fun fname -> let fhash = Elykseer_crypto.Sha256.string fname in
-                  match%lwt Relfiles.find fhash rel with None -> Lwt.return 0 | Some _ -> Lwt.return 1) fns in
-  Lwt.return @@ ((List.fold_left ((+)) 0 ls) == List.length fns)
+(* find all assembly ids in the file blocks to be restored
+   and put their encryption keys into the key store of the
+   assembly cache *)
+let ensure_keys_available (ac0 : AssemblyCache.assemblycache) relf relk fns =
+  let%lwt laids = Lwt_list.fold_left_s (fun acc fname ->
+                    let fhash = Elykseer_crypto.Sha256.string fname in
+                    match%lwt Relfiles.find fhash relf with
+                    | None -> Lwt.return acc
+                    | Some fbs ->
+                        let laids = List.map (fun (bi : Assembly.blockinformation) -> bi.blockaid) fbs.rfbs in
+                        Lwt.return (List.append laids acc)
+                  ) [] fns
+                  in
+  let lsorted = List.sort_uniq (compare) laids in
+  let%lwt kstore' = Lwt_list.fold_left_s (fun kstore aid ->
+                      match%lwt Relkeys.find aid relk with
+                      | None -> Lwt.return kstore
+                      | Some ki -> Lwt.return (Store.KeyListStore.add aid ki kstore)
+                    ) ac0.ackstore lsorted
+                    in
+  Lwt.return { ac0 with ackstore = kstore' }
 
-let restore_files e0 relf relk fns =
+let restore_files (proc0 : Processor.processor) relf relk basep fns =
     match fns with
     | [] -> Lwt.return ()
-    | _ -> if%lwt ensure_all_available e0 fns then
+    | _  -> let%lwt ac' = ensure_keys_available proc0.cache relf relk fns in
+            let proc1 = { proc0 with cache = ac'} in
               let nf = List.length fns in
-              let%lwt (cnt,_e) = Lwt_list.fold_left_s (fun (c,e) fn -> let%lwt (c',e') = restore_file e relf relk fn in Lwt.return(c + c',e')) (0,e0) fns in
+              let%lwt (cnt,_proc') = Lwt_list.fold_left_s (fun (c,proc) fn ->
+                                       let%lwt (c',proc') = restore_file proc relf relk basep fn in
+                                       Lwt.return(c + c',proc')
+                                     ) (0,proc1) fns in
               let%lwt () = if !arg_verbose then
                 Lwt_io.printlf "  restored %d files with %d bytes in total" nf cnt
                 else Lwt.return () in
               Lwt.return ()
-           else Lwt_io.printf "information on some files not found!"
 
 let exists_output_dir d =
   let dp = Filesystem.Path.from_string d in
@@ -122,8 +89,7 @@ let exists_output_dir d =
 let main () = Arg.parse argspec anon_args_fun "lxr_restore: vxodnji";
     let nchunks = Nchunks.from_int !arg_nchunks in
     if List.length !arg_files > 0
-    && !arg_nproc > 0 && !arg_nproc < 65
-    && exists_output_dir !arg_outpath
+       && exists_output_dir !arg_outpath
     then
       let myid = !arg_myid in
       let conf : configuration = {
@@ -131,10 +97,12 @@ let main () = Arg.parse argspec anon_args_fun "lxr_restore: vxodnji";
                     path_chunks = !arg_chunkpath;
                     path_db     = !arg_dbpath;
                     my_id       = myid } in
-      let e0 = Environment.EnvironmentReadable.initial_environment conf in
+      let proc = Processor.prepare_processor conf in
       let%lwt relf = Relfiles.new_map conf in
       let%lwt relk = Relkeys.new_map conf in
-      restore_files e0 relf relk !arg_files
-    else Lwt.return ()
+      let basep = Filesystem.Path.from_string !arg_outpath in
+      restore_files proc relf relk basep !arg_files
+    else
+      Lwt_io.printl "nothing to do."
 
 let () = Lwt_main.run (main ())
