elykseer-utils/actrl.ml
@@ -11,17 +11,18 @@ let create (config : Configuration.configuration) = Lwt.return {
 }
 
 let stop actrl =
-  let env = Environment.EnvironmentWritable.finalise_assembly actrl.env in
-  let%lwt relk = Relkeys.new_map env.config in
-  let%lwt () = Lwt_list.iter_s (fun (aid, ki) ->
-                                let%lwt _ = Relkeys.add aid ki relk in Lwt.return ()) env.keys.entries in
-  let%lwt () = Relkeys.close_map relk in
-  Lwt_io.printlf "stopping assembly controller %s" actrl.myid
+  match Environment.EnvironmentWritable.finalise_assembly actrl.env with
+  | None -> Lwt_io.printlf "failed to finalise assembly"
+  | Some (aid, ki) ->
+    let%lwt relk = Relkeys.new_map actrl.env.econfig in
+    let%lwt _ = Relkeys.add aid ki relk in
+    let%lwt () = Relkeys.close_map relk in
+    Lwt_io.printlf "stopping assembly controller %s" actrl.myid
 
 let addblock actrl fn (fb : Assembly.blockinformation) buf =
   (* let%lwt () = Lwt_io.printlf "adding block (%d@%d=%d) with buffer (%d)" (Conversion.p2i fb.blockid) (Conversion.n2i fb.filepos) (Conversion.n2i fb.blocksize)
                (Cstdio.File.Buffer.size buf) in *)
   let bplain = Cstdio.BufferPlain.from_buffer buf in
-  let (_apos, env') = Environment.EnvironmentWritable.backup actrl.env fn fb.filepos bplain in
-  let (_fname, fb') = List.hd @@ env'.fblocks.entries in
-  Lwt.return ({actrl with env = env'}, {fb' with blockid = fb.blockid})
+  let (env', (bi, _aki)) = Environment.EnvironmentWritable.backup actrl.env fn fb.filepos bplain in
+  (* let kstore = match aki with *)
+  Lwt.return ({actrl with env = env'}, bi)
