theories/Environment.v
@@ -23,9 +23,7 @@ Record environment (AB : Type) : RecordEnvironment :=
     mkenvironment
         { cur_assembly : assemblyinformation
         ; cur_buffer : AB
-        ; config : configuration
-        ; fblocks : FBlockListStore.R
-        ; keys : KeyListStore.R
+        ; econfig : configuration
         }.
 (* #[export] Instance etaX : Settable _ := settable! mkenvironment (AB) <cur_assembly; cur_buffer; config; fblocks; keys>. *)
 (* Print environment.
@@ -49,72 +47,54 @@ Module EnvironmentWritable <: ENV.
     Definition initial_environment (c : configuration) : E :=
         let (a,b) := AssemblyPlainWritable.create c in
         {| cur_assembly := a
-        ;  cur_buffer := b
-        ;  config := c
-        ;  fblocks := FBlockListStore.init c
-        ;  keys := KeyListStore.init c
+         ; cur_buffer := b
+         ; econfig := c
         |}.
     Definition recreate_assembly (e : environment AB) : environment AB :=
-        let (a,b) := AssemblyPlainWritable.create (e.(config AB)) in
+        let (a,b) := AssemblyPlainWritable.create (e.(econfig AB)) in
         {| cur_assembly := a; cur_buffer := b
-        ;  config := e.(config AB)
-        ;  fblocks := e.(fblocks AB)
-        ;  keys := e.(keys AB)
+        ;  econfig := e.(econfig AB)
         |}.
-    Definition env_add_file_block (fname : string) (e : environment AB) (bi : Assembly.blockinformation) : environment AB :=
-        {| cur_assembly := e.(cur_assembly AB)
-        ;  cur_buffer := e.(cur_buffer AB)
-        ;  config := e.(config AB)
-        ;  fblocks := FBlockListStore.add fname bi e.(fblocks AB)
-        ;  keys := e.(keys AB)
-        |}.
-    Definition env_add_aid_key (aid : aid_t) (e : environment AB) (ki : keyinformation) : environment AB :=
-        {| cur_assembly := e.(cur_assembly AB)
-        ;  cur_buffer := e.(cur_buffer AB)
-        ;  config := e.(config AB)
-        ;  fblocks := e.(fblocks AB)
-        ;  keys := KeyListStore.add aid ki e.(keys AB)
-        |}.
-    Definition key_for_aid (e : environment AB) (aid : Assembly.aid_t) : option keyinformation :=
-        KeyListStore.find aid e.(keys AB).
-    Definition finalise_assembly (e0 : environment AB) : environment AB :=
+    Definition finalise_assembly (e0 : environment AB) : option (aid_t * keyinformation) :=
         let a0 := e0.(cur_assembly AB) in
         let apos := Assembly.apos a0 in
         if N.ltb 0 apos then
             let (a,b) := Assembly.finish a0 e0.(cur_buffer AB) in
             let ki := {| pkey := cpp_mk_key256 tt
                        ; ivec := cpp_mk_key128 tt
-                       ; localnchunks := e0.(config AB).(Configuration.config_nchunks)
-                       ; localid := e0.(config AB).(Configuration.my_id) |} in
-            let e1 := env_add_aid_key (aid a) e0 ki in
+                       ; localnchunks := e0.(econfig AB).(Configuration.config_nchunks)
+                       ; localid := e0.(econfig AB).(Configuration.my_id) |} in
             match Assembly.encrypt a b ki with
-            | None => e0
+            | None => None
             | Some (a',b') =>
-                let n := Assembly.extract e1.(config AB) a' b' in
+                let n := Assembly.extract e0.(econfig AB) a' b' in
                 if N.ltb 0 n
-                then e1
-                else e0
+                then Some (a.(aid), ki)
+                else None
             end
-        else e0.
+        else None.
     
-    Definition finalise_and_recreate_assembly (e0 : environment AB) : environment AB :=
-        let e1 := finalise_assembly e0 in
-        EnvironmentWritable.recreate_assembly e1.
+    Definition finalise_and_recreate_assembly (e0 : environment AB) : option (environment AB * (aid_t * keyinformation)) :=
+        match finalise_assembly e0 with
+        | None => None
+        | Some ki =>
+            Some (EnvironmentWritable.recreate_assembly e0, ki)
+        end.
     
-    Program Definition backup (e0 : environment AB) (fp : string) (fpos : N) (content : BufferPlain.buffer_t) : (N * environment AB) :=
-        let afree := N.sub (Assembly.assemblysize e0.(config AB).(Configuration.config_nchunks)) e0.(cur_assembly AB).(apos) in
+    Program Definition backup (e0 : environment AB) (fp : string) (fpos : N) (content : BufferPlain.buffer_t) : (environment AB * (blockinformation * option (aid_t * keyinformation))) :=
+        let afree := N.sub (Assembly.assemblysize e0.(econfig AB).(Configuration.config_nchunks)) e0.(cur_assembly AB).(apos) in
         let blen := BufferPlain.buffer_len content in
-        let e1 := if N.ltb afree blen then
-                    finalise_and_recreate_assembly e0
-                else e0 in
+        let (ki, e1) := if N.ltb afree blen then
+                            match finalise_and_recreate_assembly e0 with
+                            | None => (None, e0)
+                            | Some (e0', ki) => (Some ki, e0')
+                            end
+                         else (None, e0) in
         let (a', bi) := Assembly.backup e1.(cur_assembly AB) e1.(cur_buffer AB) fpos content in
-        let apos := bi.(blockapos) in
-        (apos, {| cur_assembly := a'
-                ; cur_buffer := e1.(cur_buffer AB)
-                ; config := e1.(config AB)
-                ; fblocks := FBlockListStore.add fp bi e1.(fblocks AB)
-                ; keys := e1.(keys AB)
-               |}).
+        ({| cur_assembly := a'
+          ; cur_buffer := e1.(cur_buffer AB)
+          ; econfig := e1.(econfig AB)
+         |}, (bi, ki)).
 
 End EnvironmentWritable.
 (* Print EnvironmentWritable. *)
@@ -125,32 +105,17 @@ Module EnvironmentReadable <: ENV.
     Definition initial_environment (c : configuration) : E :=
         let (a,b) := AssemblyPlainFull.create c in
         {| cur_assembly := a
-        ;  cur_buffer := b
-        ;  config := c
-        ;  fblocks := FBlockListStore.init c
-        ;  keys := KeyListStore.init c
+         ; cur_buffer := b
+         ; econfig := c
         |}.
-    Definition env_add_aid_key (aid : aid_t) (e : environment AB) (ki : keyinformation) : environment AB :=
-        {| cur_assembly := e.(cur_assembly AB)
-        ;  cur_buffer := e.(cur_buffer AB)
-        ;  config := e.(config AB)
-        ;  fblocks := e.(fblocks AB)
-        ;  keys := KeyListStore.add aid ki e.(keys AB)
-        |}.
-    Definition key_for_aid (e : environment AB) (aid : Assembly.aid_t) : option keyinformation :=
-        KeyListStore.find aid e.(keys AB).
-    Definition restore_assembly (e0 : environment AB) (aid : aid_t) : option (environment AB) :=
-        match key_for_aid e0 aid with
+    Definition restore_assembly (e0 : environment AB) (aid : aid_t) (ki : keyinformation) : option (environment AB) :=
+        match Assembly.recall e0.(econfig AB) {| nchunks := e0.(econfig AB).(Configuration.config_nchunks); aid := aid; apos := 0 |} with
         | None => None
-        | Some k =>
-            match Assembly.recall e0.(config AB) {| nchunks := e0.(config AB).(Configuration.config_nchunks); aid := aid; apos := 0 |} with
+        | Some (a1, b1) =>
+            match Assembly.decrypt a1 b1 ki with
             | None => None
-            | Some (a1, b1) =>
-                match Assembly.decrypt a1 b1 k with
-                | None => None
-                | Some (a2, b2) =>
-                    Some {| cur_assembly := a2; cur_buffer := b2; config := e0.(config AB); fblocks := e0.(fblocks AB); keys := e0.(keys AB) |}
-                end
+            | Some (a2, b2) =>
+                Some {| cur_assembly := a2; cur_buffer := b2; econfig := e0.(econfig AB) |}
             end
         end.
 
